updates

Veritas.MultiSet.fst
@@ -2,9 +2,21 @@ module Veritas.MultiSet
 
 let mset (a:eqtype):Type0 = admit()
 
+let mem (#a:eqtype) (x:a) (s:mset a): Tot nat = admit()
+
 let equal (#a:eqtype) (s1:mset a) (s2:mset a): Tot bool = admit()
 
-let mem (#a:eqtype) (x:a) (s:mset a): Tot nat = admit()
+let lemma_eq_intro (#a:eqtype) (s1 s2:mset a): 
+  Lemma (requires (forall (x:a). (mem x s1 = mem x s2)))
+        (ensures (equal s1 s2)) = admit()
+
+let lemma_eq_refl (#a:eqtype) (s1 s2: mset a):
+  Lemma (requires (s1 == s2))
+        (ensures (equal s1 s2)) = admit()
+
+let lemma_eq_elim (#a:eqtype) (s1 s2: mset a):
+  Lemma (requires (equal s1 s2))
+        (ensures (s1 == s2)) = admit()
 
 (* empty set *)
 let empty (#a:eqtype): Tot (mset a) = admit()
