Veritas.MultiSet.fsti
@@ -4,18 +4,31 @@ open FStar.Seq
 
 val mset (a:eqtype): Type0
 
-val equal (#a:eqtype) (s1:mset a) (s2:mset a): Tot bool
-
 (* membership: how many copies of x are in multiset s *)
 val mem (#a:eqtype) (x:a) (s:mset a): Tot nat
+
+(* equality of two multisets *)
+val equal (#a:eqtype) (s1 s2:mset a): Tot bool
+
+val lemma_eq_intro (#a:eqtype) (s1 s2:mset a): 
+  Lemma (requires (forall (x:a). (mem x s1 = mem x s2)))
+        (ensures (equal s1 s2))
+
+val lemma_eq_refl (#a:eqtype) (s1 s2: mset a):
+  Lemma (requires (s1 == s2))
+        (ensures (equal s1 s2))
+
+val lemma_eq_elim (#a:eqtype) (s1 s2: mset a):
+  Lemma (requires (equal s1 s2))
+        (ensures (s1 == s2))
 
 (* empty set *)
 val empty (#a:eqtype): Tot (mset a)
 
 (* does a multiset contain an element x *)
-let contains (#a:eqtype) (s:mset a) (x:a) = mem x s = 0 
+let contains (#a:eqtype) (s:mset a) (x:a) = mem x s > 0 
 
-let is_empty (#a:eqtype) (s:mset a) = 
+let is_empty (#a:eqtype) (s:mset a): Tot bool = 
   equal s empty
 
 (* the empty set does not contain anything *)
